Soundness proof

src/Sound/Context.dfy
@@ -2,12 +2,13 @@ module Context {
   import opened Defs
 
     function SeqDepthExpr(ss: seq<Expr>): Idx 
+      ensures forall e <- ss :: e.Depth() <= SeqDepthExpr(ss)
     {
       if ss == [] then 0 else max(ss[0].Depth(), SeqDepthExpr(ss[1..]))
     }
 
 
-  function SeqMax(ss: seq<Idx>): Idx 
+  function  SeqMax(ss: seq<Idx>): Idx 
     ensures forall i <- ss :: i <= SeqMax(ss)
     ensures forall i: nat :: i < |ss| ==> ss[i] <= SeqMax(ss)
     ensures ss != [] ==> SeqMax(ss) in ss
@@ -17,20 +18,6 @@ module Context {
     else
       assert ss == [ss[0]] + (ss[1..]);
       max(ss[0], SeqMax(ss[1..]))
-  }
-
-  lemma MaxInsertLemma(ss: seq<Idx>, i: nat, x: Idx)
-    requires forall s <- ss :: s < x
-    requires i < |ss|
-    ensures SeqMax(ss[i := x]) == x 
-  {
-    assert forall x :: x in ss[1..] ==> x in ss;
-    assert ss[0] in ss;
-    if ss != [] {
-      if i != 0 {
-        MaxInsertLemma(ss[1..], i - 1, x);
-      }
-    }
   }
 
   datatype Context = Context(
@@ -57,8 +44,10 @@ module Context {
 
     function FreshIdx(): Idx
       ensures forall i <- incarnation :: i < FreshIdx()
+      ensures SeqDepthExpr(ctx) < FreshIdx()
+      ensures forall c <- ctx :: c.Depth() < FreshIdx()
     {
-      SeqMax(incarnation) + 1
+      max(SeqMax(incarnation), SeqDepthExpr(ctx)) + 1
     }
 
     
@@ -66,7 +55,6 @@ module Context {
     function AdjustState(s: State): State
       requires forall i <- incarnation :: i < |s|
     { 
-      // Q: how to get rid of `if`?
       seq(|incarnation|, (i: nat) requires i < |incarnation| => 
         assert incarnation[i] in incarnation;
         s[incarnation[i]])
@@ -119,11 +107,12 @@ module Context {
       ensures ctx + [Eq(BVar(vNew), Substitute(e))] == context.ctx
       ensures incarnation[v := vNew] == context.incarnation
       ensures forall i <- incarnation :: i < vNew 
-      ensures vNew == SeqMax(incarnation) + 1
-      ensures SeqMax(incarnation) + 1 == SeqMax(context.incarnation)
+      ensures forall c <- ctx :: c.Depth() < vNew
+      ensures SeqMax(incarnation) < vNew
+      ensures SeqDepthExpr(ctx) < vNew
+      // ensures 
     {
       var v' := FreshIdx();
-      MaxInsertLemma(incarnation, v, v');
       var ctx' := ctx + [Eq(BVar(v'), Substitute(e))];
       var incarnation' := incarnation[v := v'];
       context := Context(ctx', incarnation');
@@ -137,13 +126,20 @@ module Context {
     }
       
 
-    function AddVars(n: nat): Context
-      ensures incarnation <= AddVars(n).incarnation 
-      ensures AddVars(n).ctx         == ctx
-      ensures |AddVars(n).incarnation| == |incarnation| + n
+    method AddVars(n: nat) returns (ghost vNew: Idx, context: Context)
+      // ensures incarnation <= AddVars(n).incarnation 
+      ensures context.ctx         == ctx
+      ensures |context.incarnation| == |incarnation| + n
+      ensures forall i: nat :: i < n ==> context.incarnation[i] == vNew + i
+      ensures forall i: nat :: n <= i < |incarnation| + n ==> context.incarnation[i] == incarnation[i - n]
+      ensures forall c <- ctx :: c.Depth() < vNew
+      ensures SeqMax(incarnation) < vNew
+      ensures SeqDepthExpr(ctx) < vNew
     {
-      var add_on := seq(n, (i: nat) => SeqMax(incarnation) + 1 + i);
-      Context(ctx, incarnation + add_on)
+      var v := FreshIdx();
+      var addOn := seq(n, (i: nat) => v + i);
+      context := Context(ctx, addOn + incarnation);
+      vNew := v;
     }
 
     ghost predicate IsDefinedOn(d: Idx)
@@ -153,10 +149,9 @@ module Context {
 
     ghost predicate IsSatisfiedOn(s: State) 
     {
-      && IsDefinedOn(|s|) 
-      && (|s| == SeqMax(incarnation) + 1)
-      && (forall i <- incarnation :: i < |s|)
-      && (forall e <- ctx :: s.Eval(e))
+        && IsDefinedOn(|s|)
+        && (forall i <- incarnation :: i < |s|)
+        && (forall e <- ctx :: s.Eval(e))
     }
 
     ghost predicate Entails(e: Expr) 
@@ -170,6 +165,7 @@ module Context {
       requires forall ic <- incarnation :: ic + i < d
       requires i <= d
       ensures SubstituteIdx(e, i).IsDefinedOn(d)
+      ensures SubstituteIdx(e, i).Depth() <= d
       decreases e
     {
       match e 
@@ -182,6 +178,7 @@ module Context {
       requires e.IsDefinedOn(|incarnation|)
       requires forall ic <- incarnation :: ic < d
       ensures Substitute(e).IsDefinedOn(d)
+      ensures Substitute(e).Depth() <= d
       decreases e
     {
       SubstituteIdxIsDefinedOnLemma(e, 0, d);
