src/Sound/VCGen/Omni.dfy
@@ -41,11 +41,11 @@ module VCGenOmni {
       ghost var vNew;
       vNew, context := context_in.AddEq(v, x);
       VCs := [];
-      forall st: State | context_in.IsSatisfiedOn(st) 
+      forall st: State | context_in.IsSatisfiedOn(st)
         ensures Omni.SemSingle(s, context_in.AdjustState(st), context.AdjustedModels) {
         context_in.SubstituteIsDefinedOnLemma(x, |st|);
         var v' := st.Eval(context_in.Substitute(x));
-        var st' := st + [v'];
+        var st' := st.UpdateOrAdd(vNew, v');
         var stTransformed := context_in.AdjustState(st)[v := context_in.AdjustState(st).Eval(x)];
 
         assert stTransformed == context.AdjustState(st') by {
@@ -53,15 +53,16 @@ module VCGenOmni {
         }
 
         assert context.IsSatisfiedOn(st') by {
-          context_in.SubstituteIsDefinedOnLemma(x, |st'|);
+          context_in.SubstituteIsDefinedOnLemma(x, vNew);
           DepthEqLemma(BVar(vNew), context_in.Substitute(x)); 
           
           context_in.Substitute(x).EvalDepthLemma(st, st');
+
           EvalEqLemma(BVar(vNew), context_in.Substitute(x), st');
-          assert forall e: Expr :: e.IsDefinedOn(|st|) ==> 
-            st.Eval(e) ==> st'.Eval(e) by 
+
+          assert forall e <- context_in.ctx :: st.Eval(e) ==> st'.Eval(e) by 
           {
-            forall e: Expr | e.IsDefinedOn(|st|) && st.Eval(e) { 
+            forall e: Expr | e in context_in.ctx && st.Eval(e) ensures st'.Eval(e) {
               e.EvalDepthLemma(st, st');
             }
           }
@@ -97,6 +98,101 @@ module VCGenOmni {
   //     && forall i: nat :: i < |bcont| ==> posts[i] 
   // }
 
+  /**
+
+  s := s0  
+  bcont := (n1 s1); (n2 s2); (n3 s3); (n4 s4)
+
+  WP (var n3 
+        var n2 
+          var n1 s0 
+          s1 
+        s2 
+      s3) [All] ==
+  WP (var n3 
+        var n2 
+          var n1 s0 
+          s1 
+        s2) [WP(s3, All)] ==
+  WP (var n2 
+        var n1 s0 
+        s1 
+      s2) [Upd(n3, WP(s3, All)), Upd(n3, WP(s3, All))] ==
+  WP (var n2 
+        var n1 s0 
+        s1) [WP(s2, Upd(n3, WP(s3, All))), Upd(n3, WP(s3, All))] ==
+  WP (var n1 s0 
+      s1) [Upd(n2, WP(s2, Upd(n3, WP(s3, All)))), 
+           Upd(n2, WP(s2, Upd(n3, WP(s3, All)))), 
+                  Upd(n2, Upd(n3, WP(s3, All)))]] ==
+  WP (var n1 s0) 
+          [WP(s1,Upd(n2, WP(s2, Upd(n3, WP(s3, All))))), 
+                 Upd(n2, WP(s2, Upd(n3, WP(s3, All)))), 
+                  Upd(n2, Upd(n3, WP(s3, All)))]] ==
+    WP (s0) 
+          [Upd(n1, WP(s1,Upd(n2, WP(s2, Upd(n3, WP(s3, All)))))), 
+           Upd(n1, WP(s1,Upd(n2, WP(s2, Upd(n3, WP(s3, All)))))), 
+                 Upd(n1, Upd(n2, WP(s2, Upd(n3, WP(s3, All))))), 
+                 Upd(n1, Upd(n2, Upd(n3, WP(s3, All))))]] ==
+
+  
+   */
+
+  ghost function BlockWPSeq(bcont: Block.Continuation, post: iset<State>) : Omni.Continuation
+    ensures |BlockWPSeq(bcont, post)| == |bcont| + 1
+  {
+    if bcont == [] then
+      [post]
+    else 
+      var wpSeq := BlockWPSeq(bcont[1..], post);
+      var wpNew := Omni.SeqWP(bcont[0].cont, wpSeq);
+      var wpSeq := wpSeq.UpdateHead(wpNew);
+      wpSeq.UpdateAndAdd(bcont[0].varsInScope)
+  }
+
+  lemma BlockWPSeqIdx(bcont: Block.Continuation, l: nat)
+    requires l < |bcont|
+    ensures BlockWPSeq(bcont, AllStates)[l + 1] == UpdateSet(bcont.VarsInScope(l), BlockWPSeq(bcont[l..], AllStates)[0])
+  {
+    if l != 0 {
+      if |bcont| != 0 {
+        var blockWP := BlockWPSeq(bcont[1..], AllStates);
+        calc {
+          BlockWPSeq(bcont, AllStates)[l + 1];
+        ==
+          blockWP.UpdateHead(Omni.SeqWP(bcont[0].cont, blockWP)).UpdateAndAdd(bcont[0].varsInScope)[l + 1];
+        ==
+          blockWP.UpdateHead(Omni.SeqWP(bcont[0].cont, blockWP)).Update(bcont[0].varsInScope)[l];
+        == 
+          UpdateSet(bcont[0].varsInScope, blockWP.UpdateHead(Omni.SeqWP(bcont[0].cont, blockWP))[l]);
+        == { assert blockWP.UpdateHead(Omni.SeqWP(bcont[0].cont, blockWP))[l] == blockWP[l]; }
+          UpdateSet(bcont[0].varsInScope, blockWP[l]);
+        == 
+          { assert blockWP[l] == UpdateSet(bcont[1..].VarsInScope(l - 1), BlockWPSeq(bcont[l..], AllStates)[0]) by {
+              assert bcont[1..][l - 1..] == bcont[l..];
+              BlockWPSeqIdx(bcont[1..], l - 1); 
+          } }
+          UpdateSet(bcont[0].varsInScope, UpdateSet(bcont[1..].VarsInScope(l - 1), BlockWPSeq(bcont[l..], AllStates)[0]));
+        == { assert bcont.VarsInScope(l) == bcont[0].varsInScope + bcont[1..].VarsInScope(l - 1); }
+          UpdateSet(bcont.VarsInScope(l), BlockWPSeq(bcont[l..], AllStates)[0]);
+          }
+        }
+    } else {
+      calc {
+        UpdateSet(bcont.VarsInScope(0), BlockWPSeq(bcont[0..], AllStates)[0]);
+      == 
+        BlockWPSeq(bcont, AllStates)[0];
+      ==
+        BlockWPSeq(bcont, AllStates)[1];
+      }
+    }
+  }
+
+  ghost predicate BlockSem(s: seq<Stmt>, bcont: Block.Continuation, st: State, post: iset<State>) {
+    Omni.SeqSem(s, st, BlockWPSeq(bcont, post))
+  }
+
+
   method SeqVCGen(s: seq<Stmt>, context: Context, bcont: Block.Continuation) returns (VCs: seq<Expr>) 
     requires bcont.IsDefinedOn(|context.incarnation|)
 
@@ -110,12 +206,11 @@ module VCGenOmni {
     // requires SeqIsDefinedOn(s, |context.incarnation|)
     //requires bcont.IsDefinedOn(|context.incarnation|)
 
-    // ensures
-    //   (forall e <- VCs :: e.Holds()) ==> 
-    //     forall st: State:: 
-    //       context.IsSatisfiedOn(st) ==> 
-    //         && Omni.Sem(s, context.AdjustState(st), scont)
-    //         &&  Omni.SeqSem(s, context.AdjustState(st), AllStates)
+    ensures
+      (forall e <- VCs :: e.Holds()) ==> 
+        forall st: State:: 
+          context.IsSatisfiedOn(st) ==> 
+          BlockSem(s, bcont, context.AdjustState(st), AllStates)
   {
     if s == [] { 
       if bcont == [] {
@@ -126,6 +221,13 @@ module VCGenOmni {
         var cont := bcont[0].cont;
         var context' := context.Delete(varsToDelete);
         VCs := SeqVCGen(cont, context', bcont[1..]);
+        if (forall e <- VCs :: e.Holds()) {
+          forall st: State | context.IsSatisfiedOn(st)
+            ensures BlockSem([], bcont, context.AdjustState(st), AllStates) {
+            assert forall i <- context'.incarnation :: i in context.incarnation;
+            assert context'.AdjustState(st) == Tail(varsToDelete, context.AdjustState(st));
+          }
+        }
       }
     } else {
       var stmt, cont := s[0], s[1..];
@@ -134,41 +236,112 @@ module VCGenOmni {
       SeqFunConcatLemmas([stmt], cont);
       if stmt.Single() {
         var VCstmt, VCcont, context';
-        context', VCstmt := VCGen(stmt, context) by {
-            // assume {:axiom} false;
-        }
+        context', VCstmt := VCGen(stmt, context);
         VCcont := SeqVCGen(cont, context', bcont);
         VCs := VCstmt + VCcont;
+        if (forall e <- VCs :: e.Holds()) {
+          forall st: State | context.IsSatisfiedOn(st) 
+            ensures BlockSem(s, bcont, context.AdjustState(st), AllStates) {
+          }
+        }
       } else {
+        // assume {:axiom} false;
         match stmt 
         case Seq(ss) =>
           VCs := SeqVCGen(ss + cont, context, bcont) by {
             // decreases
             SeqFunConcatLemmas(ss, cont);
           }
+          if (forall e <- VCs :: e.Holds()) {
+            forall st: State | context.IsSatisfiedOn(st) 
+              ensures BlockSem(s, bcont, context.AdjustState(st), AllStates) {
+                Omni.SeqLemma(ss, cont, context.AdjustState(st), BlockWPSeq(bcont, AllStates));
+            }
+          }
         case Choice(ss0, ss1) =>
           var VCs0 := SeqVCGen([ss0] + cont, context, bcont);
           var VCs1 := SeqVCGen([ss1] + cont, context, bcont);
           VCs := VCs0 + VCs1;
+          if (forall e <- VCs :: e.Holds()) {
+            forall st: State | context.IsSatisfiedOn(st) 
+              ensures BlockSem(s, bcont, context.AdjustState(st), AllStates) {
+              
+            }
+          }
         case NewScope(n, body) =>
-          var context' := context.AddVars(n);
+          var vNew, context' := context.AddVars(n);
           VCs := SeqVCGen([body], context', bcont.Update(cont, n)) by {
             // decreases
             bcont.UpdateSize(cont, n);
             assert SeqSize([body]) == body.Size();
           }
-        case Escape(l) =>
-          var varsToDelete := bcont.VarsInScope(l);
-          var context' := context.Delete(varsToDelete) by {
-            bcont.VarsInScopeLeqAll(l);
+          if (forall e <- VCs :: e.Holds()) {
+            forall st: State | context.IsSatisfiedOn(st) 
+              ensures BlockSem(s, bcont, context.AdjustState(st), AllStates) {
+              var blockWP := BlockWPSeq(bcont, AllStates);
+              var contWP := Omni.SeqWP(cont, blockWP);
+              var updWP := ([contWP] + blockWP.UpdateHead(contWP)).Update(n);
+              assert Omni.Sem(NewScope(n, body), context.AdjustState(st), blockWP.UpdateHead(contWP)) by {
+                forall vs: State | |vs| == n 
+                  ensures Omni.Sem(body, context.AdjustState(st).Update(vs), blockWP.UpdateHead(contWP).UpdateAndAdd(n)) {
+                  var st' := st.MergeAt(vNew, vs);
+                  assert context'.IsSatisfiedOn(st') by {
+                    forall e: Expr | e in context.ctx && st.Eval(e) ensures st'.Eval(e) {
+                      e.EvalDepthLemma(st, st');
+                    }
+                  }
+                  calc {
+                    Omni.SeqSem([body], context'.AdjustState(st'), updWP);
+                  == { assert context.AdjustState(st).Update(vs) == context'.AdjustState(st'); }
+                    Omni.SeqSem([body], context.AdjustState(st).Update(vs), updWP);
+                  ==> { Omni.SeqSemSingle(body, context.AdjustState(st).Update(vs), updWP); }
+                    Omni.Sem(body, context.AdjustState(st).Update(vs), updWP);
+                  }
+                }
+              }
+              Omni.SemNest(NewScope(n, body), cont, context.AdjustState(st), blockWP);
+            }
           }
-          VCs := SeqVCGen([], context', bcont[l..]) by {
+        case Escape(l) =>
+          var bcont' := bcont.Update(cont, 0);
+          var varsToDelete := bcont'.VarsInScope(l);
+          var context' := context.Delete(varsToDelete) by {
+            bcont'.VarsInScopeLeqAll(l);
+          }
+          VCs := SeqVCGen([], context', bcont'[l..]) by {
             // decreases
-            bcont.SizePrefix(l);
+            bcont'.SizePrefix(l);
             // IsDefinedOn
-            bcont.VarsInScopeLeqAll(l);
+            bcont'.VarsInScopeLeqAll(l);
             // JumpsDefined
-            bcont.DefinedPrefix(l);
+            assert bcont'[l..].JumpsDefined() && bcont'[l..].VarsDefined() by {
+              if l != 0 {
+                assert bcont'[l..] == bcont[l - 1..];
+                bcont.DefinedPrefix(l - 1);
+              }
+            }
+          }
+          if (forall e <- VCs :: e.Holds()) {
+            forall st: State | context.IsSatisfiedOn(st)
+              ensures Omni.SeqSem([Escape(l)] + cont, context.AdjustState(st), BlockWPSeq(bcont, AllStates)) {
+              Omni.SemNest(Escape(l), cont, context.AdjustState(st), BlockWPSeq(bcont, AllStates)) by {
+                var blockWP := BlockWPSeq(bcont, AllStates);
+                var updBlockWP := blockWP.UpdateHead(Omni.SeqWP(cont, blockWP));
+                calc {
+                  context.AdjustState(st) in updBlockWP[l];
+                  { if l != 0 { BlockWPSeqIdx(bcont, l - 1); } }
+                  context.AdjustState(st) in UpdateSet(bcont'.VarsInScope(l), BlockWPSeq(bcont'[l..], AllStates)[0]);
+                  Tail(bcont'.VarsInScope(l), context.AdjustState(st)) in BlockWPSeq(bcont'[l..], AllStates)[0];
+                  { assert context'.AdjustState(st) == Tail(bcont'.VarsInScope(l), context.AdjustState(st)); }
+                  context'.AdjustState(st) in BlockWPSeq(bcont'[l..], AllStates)[0];
+                  { assert context'.IsSatisfiedOn(st) by {
+                    forall i | i in context'.incarnation ensures i < |st| {
+                      assert i in context.incarnation;
+                  } } }
+                  true;
+                }
+              }
+            }
           }
       }
     }
